change name of generated

model.v
@@ -104,21 +104,6 @@ Section MachineState.
 
 End MachineState.
   
-Section Conflict.
-  Definition write_tid_set {A : Type} (ts1 ts2 : tid -> A) : Ensemble tid :=
-    fun tid => ts1 tid <> ts2 tid.
-  Definition step_writes (s1 s2 : state) : Ensemble tid :=
-    Union tid
-          (write_tid_set s1.(commH) s2.(commH))
-          (write_tid_set s1.(Y_copy) s2.(Y_copy)).
- Definition conflict_free_step (t :tid) (s1 s2 : state) :=
-   step_writes s1 s2 = Singleton tid t /\
-   s1.(md) = s2.(md) /\
-   s1.(X_copy) = s2.(X_copy) /\
-   s1.(preH) = s2.(preH) /\
-   s1.(postH) = s2.(postH).
-End Conflict.
-
 Section Machine.
   Function combine_tid_histories (histories : tid -> history) (t : tid) :=
     match t with
@@ -181,12 +166,36 @@ Section Machine.
                   end
     end.
 
-  Inductive generated : state -> history -> Prop := (* XXX: not sure about this *)
-  | GenNil : generated start_state []
+  Inductive current_state_history : state -> history -> Prop := 
+  | GenNil : current_state_history start_state []
   | GenCons : forall s1 s2 t i r h,
                 machine_act s1 t i = (s2, (t,i,r)) ->
                 spec ((t,i,NoResp) :: h) ->
-                generated s1 h ->
-                generated s2 ((t,i,r)::h).
-
+                current_state_history s1 h ->
+                current_state_history s2 ((t,i,r)::h).
 End Machine.
+
+Section Conflict.
+  Definition write_tid_set {A : Type} (ts1 ts2 : tid -> A) : Ensemble tid :=
+    fun tid => ts1 tid <> ts2 tid.
+  Definition step_writes (s1 s2 : state) : Ensemble tid :=
+    Union tid
+          (write_tid_set s1.(commH) s2.(commH))
+          (write_tid_set s1.(Y_copy) s2.(Y_copy)).
+ Definition conflict_free_writes (t :tid) (s1 s2 : state) :=
+   step_writes s1 s2 = Singleton tid t /\
+   s1.(md) = s2.(md) /\
+   s1.(X_copy) = s2.(X_copy) /\
+   s1.(preH) = s2.(preH) /\
+   s1.(postH) = s2.(postH).
+ Definition conflict_free_reads (s s1 s2 s1' s2': state) (a1 a2: action) t i :=
+   s1.(Y_copy) t = s.(Y_copy) t ->
+   s2.(Y_copy) t = s.(Y_copy) t ->
+   s1.(commH) t = s.(commH) t ->
+   s2.(commH) t = s.(commH) t ->
+   s1.(md) = s.(md) ->
+   s2.(md) = s.(md) ->
+   machine_act s1 t i = (s1', a1) ->
+   machine_act s2 t i = (s2', a2) ->
+   a1 = a2 /\ s1'.(md) = s.(md) /\ s2'.(md) = s.(md).
+End Conflict.
